open import Utils

module FinSet
  where

open import Data.List
open import Data.Bool
open import Relation.Nullary.Decidable
open import Relation.Binary hiding (_â‡’_)
open import Data.Product
open import Data.Empty
open import Relation.Nullary
open import Relation.Binary.PropositionalEquality
open import Data.Nat renaming (_â‰Ÿ_ to _â‰Ÿâ„•_)
open import Relation.Nullary.Negation using () renaming (contradiction to _â†¯_)
open import Function
open import Data.Unit
open import Data.Sum
open import Membership

open import Induction.WellFounded

â„•-wf : Well-founded _<â€²_
â„•-wf n = acc (aux n)
  where aux : âˆ€ x y â†’ y <â€² x â†’ Acc _<â€²_ y
        aux .(suc y) y â‰¤â€²-refl = â„•-wf y
        aux .(suc x) y (â‰¤â€²-step {x} p) = aux x y p 

module WFâŠ‚mod (C : Set) (eq : DecEq C) where

  âˆ£_âˆ£ : List C â†’ â„•
  âˆ£ S âˆ£ = âˆ£ S âˆ£âŸ¨ eq âŸ© 

  open Inverse-image {_<_ = _<â€²_} (âˆ£_âˆ£) renaming (well-founded to well-founded-ii-obj)
  {- The inverse image of a well founded relation is well founded. -}
 
  _â‰º_ : List C â†’ List C â†’ Set 
  S â‰º T = S â‰ºâŸ¨ eq âŸ© T
  
  wfâ‰º : Well-founded _â‰º_
  wfâ‰º = well-founded-ii-obj â„•-wf

  _âŠ‚_ : List C â†’ List C â†’ Set
  S âŠ‚ T = S âŠ‚âŸ¨ eq âŸ© T

  âŠ‚â‡’â‰º : âˆ€ {S T} â†’ S âŠ‚ T â†’ S â‰º T
  âŠ‚â‡’â‰º (projâ‚ , projâ‚‚) = projâ‚‚
  
  open Subrelation {_<â‚_ = _âŠ‚_} {_<â‚‚_ = _â‰º_} (âŠ‚â‡’â‰º) renaming (well-founded to well-founded-sub)
  
  wfâŠ‚ : Well-founded _âŠ‚_ 
  wfâŠ‚ = well-founded-sub wfâ‰º

  comprehension-raw : (S : List C) â†’ (P : C â†’ Bool) â†’ List C
  comprehension-raw [] P = [] 
  comprehension-raw (x âˆ· S) P = let l = comprehension-raw S P
                                in if P x then (x âˆ· l) else l

  âŸªSâˆ£PâŸ«âŠ†S : âˆ€ S P â†’ comprehension-raw S P âŠ† S
  âŸªSâˆ£PâŸ«âŠ†S [] P x xâˆˆcomprehension = xâˆˆcomprehension
  âŸªSâˆ£PâŸ«âŠ†S (x âˆ· S) P xâ‚ xâˆˆcomprehension with P x
  âŸªSâˆ£PâŸ«âŠ†S (x âˆ· S) P xâ‚ xâˆˆcomprehension | false = there (âŸªSâˆ£PâŸ«âŠ†S S P xâ‚ xâˆˆcomprehension)
  âŸªSâˆ£PâŸ«âŠ†S (xâ‚ âˆ· S) P .xâ‚ here | true = here
  âŸªSâˆ£PâŸ«âŠ†S (x âˆ· S) P xâ‚ (there xâˆˆcomprehension) | true = there (âŸªSâˆ£PâŸ«âŠ†S S P xâ‚ xâˆˆcomprehension)

  xâˆˆâŸªSâˆ£PâŸ«â‡’Px : âˆ€ x S P â†’ x âˆˆ comprehension-raw S P â†’ T (P x)
  xâˆˆâŸªSâˆ£PâŸ«â‡’Px x [] P ()
  xâˆˆâŸªSâˆ£PâŸ«â‡’Px x (xâ‚ âˆ· S) P xâˆˆâŸªSâˆ£PâŸ« with P xâ‚ | inspect P xâ‚
  xâˆˆâŸªSâˆ£PâŸ«â‡’Px x (xâ‚ âˆ· S) P xâˆˆâŸªSâˆ£PâŸ« | false | hide = xâˆˆâŸªSâˆ£PâŸ«â‡’Px x S P xâˆˆâŸªSâˆ£PâŸ« 
  xâˆˆâŸªSâˆ£PâŸ«â‡’Px x (.x âˆ· S) P here | true | Reveal_Â·_is_.[ eqâ‚ ] rewrite eqâ‚ = tt
  xâˆˆâŸªSâˆ£PâŸ«â‡’Px x (xâ‚ âˆ· S) P (there xâˆˆâŸªSâˆ£PâŸ«) | true | hide = xâˆˆâŸªSâˆ£PâŸ«â‡’Px x S P xâˆˆâŸªSâˆ£PâŸ«
  
  Pxâ‡’xâˆˆSâ‡’xâˆˆâŸªSâˆ£PâŸ« : âˆ€ S P x â†’ T (P x) â†’ x âˆˆ S â†’ x âˆˆ comprehension-raw S P
  Pxâ‡’xâˆˆSâ‡’xâˆˆâŸªSâˆ£PâŸ« [] P xâ‚ TPx xâˆˆS = xâˆˆS
  Pxâ‡’xâˆˆSâ‡’xâˆˆâŸªSâˆ£PâŸ« (xâ‚ âˆ· S) P .xâ‚ TPx here with P xâ‚
  Pxâ‡’xâˆˆSâ‡’xâˆˆâŸªSâˆ£PâŸ« (xâ‚ âˆ· S) P .xâ‚ () here | false
  Pxâ‡’xâˆˆSâ‡’xâˆˆâŸªSâˆ£PâŸ« (xâ‚ âˆ· S) P .xâ‚ TPx here | true = here
  Pxâ‡’xâˆˆSâ‡’xâˆˆâŸªSâˆ£PâŸ« (x âˆ· S) P xâ‚ TPx (there xâˆˆS) with P x
  Pxâ‡’xâˆˆSâ‡’xâˆˆâŸªSâˆ£PâŸ« (x âˆ· S) P xâ‚ TPx (there xâˆˆS) | false = Pxâ‡’xâˆˆSâ‡’xâˆˆâŸªSâˆ£PâŸ« S P xâ‚ TPx xâˆˆS
  Pxâ‡’xâˆˆSâ‡’xâˆˆâŸªSâˆ£PâŸ« (x âˆ· S) P xâ‚ TPx (there xâˆˆS) | true = there (Pxâ‡’xâˆˆSâ‡’xâˆˆâŸªSâˆ£PâŸ« S P xâ‚ TPx xâˆˆS)
  
  comprehension-syntax : âˆ€ (S : List C) â†’ (P : C â†’ Bool) â†’ List C
  comprehension-syntax S P = projâ‚ (dedup eq (comprehension-raw S P))

  syntax comprehension-raw S (Î» x â†’ B) = âŸª x âˆˆ S âˆ£ B âŸ«

  _âŠ‚?_ : (S : List C) â†’ (T : List C) â†’ Dec (S âŠ‚ T)
  S âŠ‚? T = S âŠ‚âŸ¨ eq âŸ©? T

  _âˆˆ?_ : (x : C) â†’ (L : List C) â†’ Dec (x âˆˆ L)
  x âˆˆ? S = eq2in eq x S

  _âˆ©_ : List C â†’ List C â†’ List C
  S âˆ© T = âŸª s âˆˆ S âˆ£ âŒŠ s âˆˆ? T âŒ‹ âŸ«

  _Ì¸_ : List C â†’ List C â†’ List C
  S Ì¸ T = âŸª s âˆˆ S âˆ£ not âŒŠ s âˆˆ? T âŒ‹ âŸ« 

  ð“œ : C â†’ List C â†’ â„• 
  ð“œ x S = multiplicity eq x S

  _âŸ¶_ : âˆ€ (P Q : C â†’ Bool) â†’ Set
  P âŸ¶ Q = âˆ€ {s : C} â†’ T (P s) â†’ T (Q s)

  BoolImp : âˆ€ (P Q : C â†’ Bool) â†’ âˆ€ (s : C) â†’ T (P s â‡’ Q s) â†’ T (P s) â†’ T (Q s)
  BoolImp P Q s Psâ‡’Qs Ps with P s | Q s
  BoolImp P Q s Psâ‡’Qs () | false | Qs
  BoolImp P Q s () Ps | true | false
  BoolImp P Q s Psâ‡’Qs Ps | true | true = tt

  ImpBool : âˆ€ (P Q : C â†’ Bool) â†’ âˆ€ (s : C) â†’ (T (P s) â†’ T (Q s)) â†’ T (P s â‡’ Q s) 
  ImpBool P Q s Psâ‡’Qs with P s | Q s 
  ImpBool P Q s Psâ‡’Qs | false | Qs = tt
  ImpBool P Q s Psâ‡’Qs | true | Qs = Psâ‡’Qs tt
  
  ImplicationLawRaw : âˆ€ (S : List C) â†’ (P Q : C â†’ Bool) â†’ P âŸ¶ Q â†’ comprehension-raw S P âŠ† comprehension-raw S Q 
  ImplicationLawRaw [] P Q imp x ()
  ImplicationLawRaw (x âˆ· S) P Q imp xâ‚ inS with ImpBool P Q x (imp {x})
  ImplicationLawRaw (x âˆ· S) P Q imp xâ‚ inS | ix with P x | Q x
  ImplicationLawRaw (x âˆ· S) P Q imp xâ‚ inS | ix | false | false = ImplicationLawRaw S P Q imp xâ‚ inS
  ImplicationLawRaw (x âˆ· S) P Q imp xâ‚ inS | ix | false | true = there $ ImplicationLawRaw S P Q imp xâ‚ inS
  ImplicationLawRaw (x âˆ· S) P Q imp xâ‚ inS | () | true | false
  ImplicationLawRaw (xâ‚ âˆ· S) P Q imp .xâ‚ here | ix | true | true = here
  ImplicationLawRaw (x âˆ· S) P Q imp xâ‚ (there inS) | ix | true | true = there $ ImplicationLawRaw S P Q imp xâ‚ inS

  ImplicationLaw : âˆ€ (S : List C) â†’ (P Q : C â†’ Bool) â†’ P âŸ¶ Q â†’ comprehension-syntax S P âŠ† comprehension-syntax S Q
  ImplicationLaw S P Q imp x inS = dedup-complete eq (comprehension-raw S Q) x (ImplicationLawRaw S P Q imp x (dedup-sound eq (comprehension-raw S P) x inS))

  ComprehensionMonotone : âˆ€ (S R : List C) â†’ (P Q : C â†’ Bool) â†’ S âŠ† R â†’ P âŸ¶ Q â†’ comprehension-raw S P âŠ† comprehension-raw R Q
  ComprehensionMonotone S R P Q SâŠ†R PâŸ¶Q x xâˆˆâŸªSâˆ£PâŸ© =
    let xâˆˆS = âŸªSâˆ£PâŸ«âŠ†S S P x xâˆˆâŸªSâˆ£PâŸ©
        xâˆˆR = SâŠ†R x xâˆˆS
        Px = xâˆˆâŸªSâˆ£PâŸ«â‡’Px x S P xâˆˆâŸªSâˆ£PâŸ©
        Qx = PâŸ¶Q Px 
        xâˆˆâŸªRâˆ£QâŸ« = Pxâ‡’xâˆˆSâ‡’xâˆˆâŸªSâˆ£PâŸ« R Q x Qx xâˆˆR
     in xâˆˆâŸªRâˆ£QâŸ«
  
  BothIntersection : âˆ€ {A B x} â†’ (x âˆˆ A) â†’ (x âˆˆ B) â†’ x âˆˆ (A âˆ© B)
  BothIntersection {x âˆ· A} {B} here xâˆˆB with x âˆˆ? B
  BothIntersection {x âˆ· A} here xâˆˆB | yes p = here
  BothIntersection {x âˆ· A} here xâˆˆB | no Â¬p = xâˆˆB â†¯ Â¬p
  BothIntersection {x âˆ· A} (there xâˆˆA) xâˆˆB with BothIntersection xâˆˆA xâˆˆB
  BothIntersection {x âˆ· A} {B} (there xâˆˆA) xâˆˆB | res with x âˆˆ? B
  BothIntersection {x âˆ· A} (there xâˆˆA) xâˆˆB | res | yes p = there res
  BothIntersection {x âˆ· A} (there xâˆˆA) xâˆˆB | res | no Â¬p = res

  IntersectionBoth : âˆ€ {A B x} â†’ x âˆˆ (A âˆ© B) â†’ (x âˆˆ A) Ã— (x âˆˆ B) 
  IntersectionBoth {[]} ()
  IntersectionBoth {x âˆ· A} {B} inboth with x âˆˆ? B
  IntersectionBoth {x âˆ· A} here | yes p = here , p
  IntersectionBoth {x âˆ· A} (there inboth) | yes p = let xâˆˆAÃ—xâˆˆB = IntersectionBoth {A} inboth
                                                    in there (projâ‚ xâˆˆAÃ—xâˆˆB)  , (projâ‚‚ xâˆˆAÃ—xâˆˆB)
  IntersectionBoth {x âˆ· A} inboth | no Â¬p = let xâˆˆAÃ—xâˆˆB = IntersectionBoth {A} inboth
                                            in there (projâ‚ xâˆˆAÃ—xâˆˆB)  , (projâ‚‚ xâˆˆAÃ—xâˆˆB)

  IntersectionLaw : âˆ€ {A B C D} â†’ A âŠ† B â†’ C âŠ† D â†’ (A âˆ© C) âŠ† (B âˆ© D)
  IntersectionLaw {A} AâŠ†B CâŠ†D x xin =
    let (xâˆˆA , xâˆˆC) = IntersectionBoth {A} xin
    in let xâˆˆB = AâŠ†B x xâˆˆA
       in let xâˆˆD = CâŠ†D x xâˆˆC
           in BothIntersection xâˆˆB xâˆˆD 

  IntersectionLeft : âˆ€ {A B C} â†’ A âŠ† C â†’ (A âˆ© B) âŠ† C
  IntersectionLeft {A} AâŠ†C x xâˆˆAâˆ©B with IntersectionBoth {A} xâˆˆAâˆ©B
  IntersectionLeft AâŠ†C x xâˆˆAâˆ©B | xâˆˆA , xâˆˆB = AâŠ†C x xâˆˆA

  IntersectionRight : âˆ€ {A B C} â†’ B âŠ† C â†’ (A âˆ© B) âŠ† C
  IntersectionRight {A} BâŠ†C x xâˆˆAâˆ©B with IntersectionBoth {A} xâˆˆAâˆ©B
  IntersectionRight BâŠ†C x xâˆˆAâˆ©B | xâˆˆA , xâˆˆB = BâŠ†C x xâˆˆB

  BoolSub : âˆ€ {A B t} â†’ A âŠ† B â†’ T âŒŠ t âˆˆ? A âŒ‹ â†’ T âŒŠ t âˆˆ? B âŒ‹
  BoolSub {A} {B} {t} sub tâˆˆ?A with t âˆˆ? A
  BoolSub {A} {B} {t} sub tâˆˆ?A | yes p with t âˆˆ? B
  BoolSub sub tâˆˆ?A | yes pâ‚ | yes p = tt
  BoolSub sub tâˆˆ?A | yes p | no Â¬p = sub _ p â†¯ Â¬p  
  BoolSub sub () | no Â¬p
  
  OrIntroL : âˆ€ {P R} â†’ T R â†’ T (P âˆ¨ R)
  OrIntroL {R = false} ()
  OrIntroL {false} {true} TR = tt
  OrIntroL {true} {true} TR = tt 

  AndIntro : âˆ€ {P Q} â†’ T P â†’ T Q â†’ T (P âˆ§ Q)
  AndIntro {false} Tp Tq = Tp
  AndIntro {true} Tp Tq = Tq

  ImplyAnd : âˆ€ {P Q R} â†’ (T Q â†’ T R) â†’ T (P âˆ§ Q) â†’ T (P âˆ§ R)
  ImplyAnd {false} TQâ‡’TR ()
  ImplyAnd {true} TQâ‡’TR Pâˆ§Q = TQâ‡’TR Pâˆ§Q

  ImpliesExists : âˆ€ S P Q â†’ P âŸ¶ Q â†’ T (any P S) â†’ T (any Q S)
  ImpliesExists [] P Q PâŸ¶Q âˆƒtâˆˆS = âˆƒtâˆˆS
  ImpliesExists (x âˆ· S) P Q PâŸ¶Q âˆƒtâˆˆS with PâŸ¶Q {x}
  ImpliesExists (x âˆ· S) P Q PâŸ¶Q âˆƒtâˆˆS | f with P x
  ImpliesExists (x âˆ· S) P Q PâŸ¶Q âˆƒtâˆˆS | f | false with ImpliesExists S P Q PâŸ¶Q âˆƒtâˆˆS 
  ImpliesExists (x âˆ· S) P Q PâŸ¶Q âˆƒtâˆˆS | f | false | anyS = OrIntroL {Q x} anyS
  ImpliesExists (x âˆ· S) P Q PâŸ¶Q âˆƒtâˆˆS | f | true with f tt
  ImpliesExists (x âˆ· S) P Q PâŸ¶Q âˆƒtâˆˆS | f | true | TQx with Q x
  ImpliesExists (x âˆ· S) P Q PâŸ¶Q âˆƒtâˆˆS | f | true | () | false
  ImpliesExists (x âˆ· S) P Q PâŸ¶Q âˆƒtâˆˆS | f | true | TQx | true = tt

  ImpliesAll : âˆ€ S P Q â†’ P âŸ¶ Q â†’ T (all P S) â†’ T (all Q S)
  ImpliesAll [] P Q PâŸ¶Q Î tâˆˆS = tt
  ImpliesAll (x âˆ· S) P Q PâŸ¶Q Î tâˆˆS with PâŸ¶Q {x}
  ImpliesAll (x âˆ· S) P Q PâŸ¶Q Î tâˆˆS | f with P x
  ImpliesAll (x âˆ· S) P Q PâŸ¶Q () | f | false
  ImpliesAll (x âˆ· S) P Q PâŸ¶Q Î tâˆˆS | f | true with ImpliesAll S P Q PâŸ¶Q Î tâˆˆS
  ImpliesAll (x âˆ· S) P Q PâŸ¶Q Î tâˆˆS | f | true | allS with f tt
  ImpliesAll (x âˆ· S) P Q PâŸ¶Q Î tâˆˆS | f | true | allS | TQx = AndIntro TQx allS

  LessEmptyIsEmpty : âˆ€ {A : List C} â†’ A âŠ† [] â†’ A â‰¡ []
  LessEmptyIsEmpty {[]} p = refl
  LessEmptyIsEmpty {x âˆ· A} p with p x here
  LessEmptyIsEmpty {x âˆ· A} p | ()

  NegationLaw : âˆ€ S {A B} â†’ A âŠ† B â†’ (S Ì¸ B) âŠ† (S Ì¸ A)
  NegationLaw [] AâŠ†B x xâˆˆSÌ¸B = xâˆˆSÌ¸B
  NegationLaw (x âˆ· S) {A} {B} AâŠ†B with x âˆˆ? A
  NegationLaw (x âˆ· S) {A} {B} AâŠ†B | yes p with AâŠ†B x p
  NegationLaw (x âˆ· S) {A} {B} AâŠ†B | yes p | res with x âˆˆ? B
  NegationLaw (x âˆ· S) AâŠ†B | yes pâ‚ | res | yes p = NegationLaw S AâŠ†B
  NegationLaw (x âˆ· S) AâŠ†B | yes p | res | no Â¬p = res â†¯ Â¬p
  NegationLaw (x âˆ· S) {A} {B} AâŠ†B | no Â¬p with x âˆˆ? B
  NegationLaw (x âˆ· S) AâŠ†B | no Â¬p | yes p = Î» y yâˆˆSÌ¸B â†’ there $ NegationLaw S AâŠ†B y yâˆˆSÌ¸B
  NegationLaw (x âˆ· S) AâŠ†B | no Â¬pâ‚ | no Â¬p with NegationLaw S AâŠ†B
  NegationLaw (x âˆ· S) AâŠ†B | no Â¬pâ‚ | no Â¬p | res = Î» y yâˆˆSÌ¸B â†’ hereOrThere S AâŠ†B yâˆˆSÌ¸B
    where hereOrThere : âˆ€ S {A B x y} â†’ A âŠ† B â†’ y âˆˆ (x âˆ· (S Ì¸ B)) â†’ y âˆˆ (x âˆ· (S Ì¸ A))
          hereOrThere S AâŠ†B here = here
          hereOrThere S AâŠ†B (there yâˆˆSÌ¸B) = there $ NegationLaw S AâŠ†B _ yâˆˆSÌ¸B

  open import Database C C eq eq

  ImpliesAbstract : âˆ€ {P Q R} â†’ T (Q â‡’ R) â†’ T (P â‡’ Q) â†’ T (P â‡’ R)
  ImpliesAbstract {false} Qâ‡’R Pâ‡’R = tt
  ImpliesAbstract {true} {false} Qâ‡’R ()
  ImpliesAbstract {true} {true} Qâ‡’R Pâ‡’R = Qâ‡’R
